\documentclass[12pt, letterpaper]{article}
\usepackage{amsmath}
\usepackage{tensor}
\usepackage{stix}
\usepackage{graphicx} % Required for inserting images
%\usepackage[paperheight=6in,
%   paperwidth=5in,
%   top=10mm,
%   bottom=20mm,
%   left=10mm,
%   right=10mm]{geometry}
\newcommand*{\1}{\hspace{1pt}}
\title{Solution to Problem Sheet 2}
\author{Noor E Mustafa Ferdous}
\date{}

\begin{document}

\maketitle

\section*{Solve for problem no. 1}
Given

\begin{equation}
    \left\{ \gamma ^{\mu}, \gamma ^{\nu} \right\} = 2 \eta ^{\mu \nu}    
\end{equation}

From L.H.S. 

\begin{align*}
    \left[ \gamma ^{\kappa} \gamma ^{\lambda}, \gamma ^{\mu} \gamma ^{\nu} \right] &= \gamma ^{\kappa} \left[ \gamma ^{\lambda}, \gamma ^{\mu} \gamma ^{\nu}\right] + \left[\gamma ^{\kappa}, \gamma ^{\mu} \gamma ^{\nu}\right] \gamma ^{\lambda} \\ 
    &= \gamma ^{\kappa} \left( \gamma ^{\lambda}\gamma ^{\mu} \gamma ^{\nu} - \gamma ^{\mu} \gamma ^{\nu}\gamma ^{\lambda}\right) + \left(\gamma ^{\kappa}\gamma ^{\mu} \gamma ^{\nu} - \gamma ^{\mu} \gamma ^{\nu} \gamma ^{\kappa}\right)\gamma ^{\lambda} \\ 
    &= \gamma ^{\kappa} \left( \left(\gamma ^{\lambda}\gamma ^{\mu} + \gamma ^{\mu}\gamma ^{\lambda}\right) \gamma ^{\nu} - \gamma ^{\mu} \left( \gamma ^{\lambda} \gamma ^{\nu} + \gamma ^{\nu} \gamma ^{\lambda} \right) + \left( \left(\gamma ^{\kappa}\gamma ^{\mu} +\gamma ^{\mu}\gamma ^{\kappa}\right) \gamma ^{\nu} - \gamma ^{\mu} \left(\gamma ^{\nu} \gamma ^{\kappa} + \gamma ^{\kappa} \gamma ^{\nu} \right) \right)\gamma ^{\lambda}\right) \\
    &= \gamma ^{\kappa} \left(\left( \left\{ \gamma ^{\lambda}, \gamma ^{\mu} \right\} \gamma ^{\nu} - \gamma ^{\mu} \left\{ \gamma ^{\lambda}, \gamma ^{\nu} \right\} \right) + \left( \left\{ \gamma ^{\kappa}, \gamma ^{\mu} \right\} \gamma ^{\nu} - \gamma ^{\mu} \left\{\gamma ^{\nu}, \gamma ^{\kappa} \right\} \right)\gamma ^{\lambda}\right) \\
   \left[ \gamma ^{\kappa} \gamma ^{\lambda}, \gamma ^{\mu} \gamma ^{\nu} \right] &= 2\eta ^{\lambda \mu} \gamma ^{\kappa} \gamma ^{\nu} - 2\eta ^{\lambda \nu} \gamma ^{\kappa} \gamma \mu + 2\eta ^{\kappa \mu} \gamma ^{\nu} \gamma ^{\lambda} - 2\eta ^{\nu \kappa} \gamma ^{\mu} \gamma ^{\lambda} \tag{Showed}
\end{align*}


\begin{align*}
	(a) \ Tr(\gamma ^{\mu}) &= Tr(\gamma ^{\mu} \gamma _{5} \gamma _{5}) \tag{[because $(\gamma _{5})^{2} = 1]$} \\
	&= - Tr(\gamma _{5} \gamma ^{\mu} \gamma _{5}) = - Tr(\gamma _{5} \gamma ^{\mu} \gamma _{5}) \\ 
	\implies  Tr(\gamma ^{\mu} \gamma _{5} \gamma _{5}) &= - Tr(\gamma _{5} \gamma ^{\mu} \gamma _{5}) = Tr(\gamma _{5} \gamma ^{\mu} \gamma _{5}) \\ 
	 Tr(\gamma ^{\mu} \gamma _{5} \gamma _{5}) &= 0 \\
	 \implies Tr(\gamma ^{\mu}) = 0
\end{align*}

\begin{align*}
    (b) \ Tr(\gamma ^{\mu} \gamma ^{\nu}) &= \frac{1}{2}\left(Tr(\gamma ^{\mu} \gamma ^{\nu}) + Tr(\gamma ^{\mu} \gamma ^{\nu}) \right) \\ 
    &= \frac{1}{2}\left(Tr(\gamma ^{\mu} \gamma ^{\nu}) + Tr(\gamma ^{\nu} \gamma ^{\mu}) \right) \\
    &= \frac{1}{2}\left(Tr(\gamma ^{\mu} \gamma ^{\nu} + \gamma ^{\nu} \gamma ^{\mu}) \right) \\
    &= \frac{1}{2} Tr \left\{ \gamma ^{\mu}, \gamma ^{\nu}\right\} \\ 
    &= \frac{1}{2} Tr 2 \eta ^{\mu \nu} \\ 
    &= \frac{1}{2} 2 \eta ^{\mu \nu} Tr(\mathbb{1}) \\
    &= 4 \eta ^{\mu \nu}
\end{align*}

\begin{align*}
    (d) \ (\gamma ^{5}) ^{2} &= i \gamma _{0} \gamma _{1} \gamma _{2} \gamma _{3} \cdot i \gamma _{0} \gamma _{1} \gamma _{2} \gamma _{3} \\
    &= - (-1) \gamma _{0} \gamma _{0} \gamma _{1} \gamma _{2} \gamma _{3} \gamma _{1} \gamma _{2} \gamma _{3} \\ 
    &= \gamma _{1} \gamma _{2} \gamma _{3}\gamma _{1} \gamma _{2} \gamma _{3} \\ 
    &= \gamma _{1} \gamma _{1} \gamma _{2} \gamma _{3} \gamma _{2} \gamma _{3} 
    &= - \gamma _{2} \gamma _{3}\gamma _{2} \gamma _{3} \\ 
    &= \gamma _{2} \gamma _{2} \gamma _{3}\gamma _{3} \\ 
    &= 1
\end{align*}

\begin{align*}
    (e) \ Tr (\gamma ^{5}) &= Tr (\gamma ^{5} \gamma ^{0} \gamma ^{0}) \tag{$(\gamma ^{0})^{2} = 1$} \\
    &= - Tr(\gamma ^{0} \gamma ^{5} \gamma {0}) = Tr(\gamma ^{0} \gamma ^{5} \gamma {0}) = 0
\end{align*}

\section*{Solution to problem 2}

Given,

\begin{equation}
    \psi (\overrightarrow{x} ) = \sum_{s = 1}^{2} \int \frac{d ^{3} p}{(2 \pi) ^{3}} \frac{1}{\sqrt{2 E _{\overrightarrow{p}}}} \left[b^{s} _{\overrightarrow{p}}u^{s}(\overrightarrow{p}) e ^{i \overrightarrow{p} \cdot \overrightarrow{x}} + c^{s \dagger} _{\overrightarrow{p}}v^{s}(\overrightarrow{p}) e ^{ - i \overrightarrow{p} \cdot \overrightarrow{x}}\right]  
\end{equation}

And

\begin{equation}
    \psi ^{\dagger} (\overrightarrow{x} ) = \sum_{s = 1}^{2} \int \frac{d ^{3} p}{(2 \pi) ^{3}} \frac{1}{\sqrt{2 E _{\overrightarrow{p}}}} \left[b^{s \dagger} _{\overrightarrow{p}}u^{s \dagger}(\overrightarrow{p}) e ^{-i \overrightarrow{p} \cdot \overrightarrow{x}} + c^{s} _{\overrightarrow{p}}v^{s \dagger}(\overrightarrow{p}) e ^{i \overrightarrow{p} \cdot \overrightarrow{x}}\right]  
\end{equation}

Now
\begin{align*}
	&\left\{ \psi _{\alpha} (\overrightarrow{x}) , \psi ^{\dagger} _{\beta }(\overrightarrow{y})  \right\}  \\
	&= \bigg\{\sum_{\alpha = 1}^{4}\sum_{s = 1}^{2} \int \frac{d ^{3} p}{(2 \pi) ^{3}} \frac{d ^{3} p ^{\prime}}{(2 \pi) ^{3}}\frac{1}{\sqrt{2 E _{\overrightarrow{p}}}} \left[b^{s} _{\overrightarrow{p}}u^{s} _{\alpha}(\overrightarrow{p}) e ^{i \overrightarrow{p} \cdot \overrightarrow{x}} + c^{s \dagger} _{\overrightarrow{p}}v^{s} _{\alpha}(\overrightarrow{p}) e ^{ - i \overrightarrow{p} \cdot \overrightarrow{x}}\right], \\
    & \sum_{\beta = 1}^{4} \sum_{r = 1}^{2} \int \frac{d ^{3} p^{\prime}}{(2 \pi) ^{3}}\frac{d ^{3} p ^{\prime}}{(2 \pi) ^{3}} \frac{1}{\sqrt{2 E _{\overrightarrow{p^{\prime}}}}} \left[b^{r \dagger} _{\overrightarrow {p ^{\prime}}}u^{r \dagger} _{\beta}(\overrightarrow{p ^{\prime}}) e ^{-i \overrightarrow{p^{\prime}} \cdot \overrightarrow{y}} + c^{r} _{\overrightarrow{p ^{\prime}}}v^{r \dagger} _{\beta}(\overrightarrow{p ^{\prime}}) e ^{i \overrightarrow{p ^{\prime}} \cdot \overrightarrow{y}}\right] \bigg\} \\
    &= \sum_{\alpha = 1}^{4}\sum_{\beta = 1}^{4} \sum_{s = 1}^{2} \sum_{r = 1}^{2} \int \frac{d ^{3} p}{(2 \pi) ^{3}}\frac{d ^{3} p ^{\prime}}{(2 \pi) ^{3}} \frac{1}{\sqrt{2 E _{\overrightarrow{p}}}} \frac{1}{\sqrt{2 E _{\overrightarrow{p^{\prime}}}}}\bigg[b^{s} _{\overrightarrow{p}}u^{s} _{\alpha}(\overrightarrow{p})b^{r \dagger} _{\overrightarrow {p ^{\prime}}}u^{r \dagger} _{\beta}(\overrightarrow{p ^{\prime}}) e ^{i \overrightarrow{p} \cdot \overrightarrow{x} -i \overrightarrow{p^{\prime}} \cdot \overrightarrow{y}} + b^{s} _{\overrightarrow{p}}u^{s} _{\alpha}(\overrightarrow{p})c^{r} _{\overrightarrow{p ^{\prime}}}v^{r \dagger} _{\beta}(\overrightarrow{p ^{\prime}})e ^{i \overrightarrow{p} \cdot \overrightarrow{x} + i \overrightarrow{p^{\prime}} \cdot \overrightarrow{y}} \\
    & + c^{s \dagger} _{\overrightarrow{p}}v^{s} _{\alpha}(\overrightarrow{p}) b^{r \dagger} _{\overrightarrow {p ^{\prime}}}u^{r \dagger} _{\beta}(\overrightarrow{p ^{\prime}})  e ^{-i \overrightarrow{p} \cdot \overrightarrow{x} -i \overrightarrow{p^{\prime}} \cdot \overrightarrow{y}} + c^{s \dagger} _{\overrightarrow{p}}v^{s} _{\alpha}(\overrightarrow{p}) c^{r} _{\overrightarrow{p ^{\prime}}}v^{r \dagger} _{\beta}(\overrightarrow{p ^{\prime}}) e ^{- i \overrightarrow{p} \cdot \overrightarrow{x} + i \overrightarrow{p^{\prime}} \cdot \overrightarrow{y}} + b^{r \dagger} _{\overrightarrow {p ^{\prime}}}u^{r \dagger} _{\beta}(\overrightarrow{p ^{\prime}}) b^{s} _{\overrightarrow{p}}u^{s} _{\alpha}(\overrightarrow{p})e ^{i \overrightarrow{p} \cdot \overrightarrow{x} -i \overrightarrow{p^{\prime}} \cdot \overrightarrow{y}} \\
    & + c^{r} _{\overrightarrow{p ^{\prime}}}v^{r \dagger} _{\beta}(\overrightarrow{p ^{\prime}})b^{s} _{\overrightarrow{p}}u^{s} _{\alpha}(\overrightarrow{p})e ^{i \overrightarrow{p} \cdot \overrightarrow{x} + i \overrightarrow{p^{\prime}} \cdot \overrightarrow{y}} + b^{r \dagger} _{\overrightarrow {p ^{\prime}}}u^{r \dagger} _{\beta}(\overrightarrow{p ^{\prime}}) c^{s \dagger} _{\overrightarrow{p}}v^{s} _{\alpha}(\overrightarrow{p}) e ^{-i \overrightarrow{p} \cdot \overrightarrow{x} -i \overrightarrow{p^{\prime}} \cdot \overrightarrow{y}} + c^{s \dagger} _{\overrightarrow{p}}v^{s} _{\alpha}(\overrightarrow{p}) c^{r} _{\overrightarrow{p ^{\prime}}}v^{r \dagger} _{\beta}(\overrightarrow{p ^{\prime}}) e ^{-i \overrightarrow{p} \cdot \overrightarrow{x} +i \overrightarrow{p^{\prime}} \cdot \overrightarrow{y}} \bigg]\\ 
\end{align*}
\begin{align}
    \begin{split}    
    & = \sum_{\alpha = 1}^{4}\sum_{\beta = 1}^{4} \sum_{s = 1}^{2} \sum_{r = 1}^{2} \int \frac{d ^{3} p}{(2 \pi) ^{3}} \frac{d ^{3} p ^{\prime}}{(2 \pi) ^{3}} \frac{1}{\sqrt{2 E _{\overrightarrow{p}}}} \frac{1}{\sqrt{2 E _{\overrightarrow{p^{\prime}}}}}\bigg[ \big\{b^{s} _{\overrightarrow{p}}, b^{r \dagger} _{\overrightarrow {p ^{\prime}}}\big\} u^{s} _{\alpha}(\overrightarrow{p})u^{r \dagger} _{\beta}(\overrightarrow{p ^{\prime}})e ^{i \overrightarrow{p} \cdot \overrightarrow{x} -i \overrightarrow{p^{\prime}} \cdot \overrightarrow{y}} + \big\{b^{s} _{\overrightarrow{p}}, c^{r \dagger} _{\overrightarrow {p ^{\prime}}}\big\}u^{s} _{\alpha}(\overrightarrow{p})v^{r \dagger} _{\beta}(\overrightarrow{p ^{\prime}})e ^{i \overrightarrow{p} \cdot \overrightarrow{x} + i \overrightarrow{p^{\prime}} \cdot \overrightarrow{y}} \\
    &+ \big\{c^{s} _{\overrightarrow{p}}, b^{r \dagger} _{\overrightarrow {p ^{\prime}}}\big\}v^{s} _{\alpha}(\overrightarrow{p})u^{r \dagger} _{\beta}(\overrightarrow{p ^{\prime}})e ^{-i \overrightarrow{p} \cdot \overrightarrow{x} - i \overrightarrow{p^{\prime}} \cdot \overrightarrow{y}}  + \big\{c^{s} _{\overrightarrow{p}}, c^{r \dagger} _{\overrightarrow {p ^{\prime}}}\big\}v^{s} _{\alpha}(\overrightarrow{p})v^{r \dagger} _{\beta}(\overrightarrow{p ^{\prime}})e ^{-i \overrightarrow{p} \cdot \overrightarrow{x} + i \overrightarrow{p^{\prime}} \cdot \overrightarrow{y}} 
    \end{split}
\end{align}

Given 

\begin{equation}
    \big\{b^{s} _{\overrightarrow{p}}, b^{r} _{\overrightarrow {p ^{\prime}}}\big\} = \big\{c^{s} _{\overrightarrow{p}}, c^{r } _{\overrightarrow {p ^{\prime}}}\big\} = \big\{c^{s} _{\overrightarrow{p}}, b^{r \dagger} _{\overrightarrow {p ^{\prime}}}\big\} = \big\{c^{s} _{\overrightarrow{p}}, b^{r} _{\overrightarrow {p ^{\prime}}}\big\} = ..... = 0
\end{equation}

\begin{equation}
    \big\{b^{s} _{\overrightarrow{p}}, b^{r \dagger} _{\overrightarrow {p ^{\prime}}}\big\} = \big\{c^{s} _{\overrightarrow{p}}, c^{r \dagger} _{\overrightarrow {p ^{\prime}}}\big\} = (2 \pi) ^{3} \delta ^{rs} \delta ^{(3)}(\overrightarrow{p} - \overrightarrow{p ^{\prime}}) 
\end{equation}

Therefore eqn(4) will be 
\begin{align*}
    &\left\{ \psi _{\alpha} (\overrightarrow{x}) , \psi ^{\dagger} _{\beta }(\overrightarrow{y})  \right\} =  \\
    & \sum_{\alpha = 1}^{4}\sum_{\beta = 1}^{4} \sum_{s = 1}^{2} \sum_{r = 1}^{2} \int \frac{d ^{3} p}{(2 \pi) ^{3}}\frac{d ^{3} p ^{\prime}}{(2 \pi) ^{3}} \frac{1}{\sqrt{2 E _{\overrightarrow{p}}}} \frac{1}{\sqrt{2 E _{\overrightarrow{p^{\prime}}}}}\bigg[ (2 \pi) ^{3} \delta ^{rs} \delta ^{(3)}(\overrightarrow{p} - \overrightarrow{p ^{\prime}}) u^{s} _{\alpha}(\overrightarrow{p})u^{r \dagger} _{\beta}(\overrightarrow{p ^{\prime}})e ^{i \overrightarrow{p} \cdot \overrightarrow{x} -i \overrightarrow{p^{\prime}} \cdot \overrightarrow{y}} \\
    & + (2 \pi) ^{3} \delta ^{rs} \delta ^{(3)}(\overrightarrow{p} - \overrightarrow{p ^{\prime}}) v^{s} _{\alpha}(\overrightarrow{p})v^{r \dagger} _{\beta}(\overrightarrow{p ^{\prime}})e ^{-i \overrightarrow{p} \cdot \overrightarrow{x} +i \overrightarrow{p^{\prime}} \cdot \overrightarrow{y}} \bigg] \\
    &= \sum_{\alpha = 1}^{4}\sum_{\beta = 1}^{4} \int \frac{d ^{3} p}{(2 \pi) ^{6}} \frac{1}{{2 E _{\overrightarrow{p}}}} \bigg[ (2 \pi) ^{3} u _{\alpha}(\overrightarrow{p})u^{\dagger} _{\beta}(\overrightarrow{p})e ^{i \overrightarrow{p} \cdot (\overrightarrow{x} - \overrightarrow{y})} + (2 \pi) ^{3} v _{\alpha}(\overrightarrow{p})v^{\dagger} _{\beta}(\overrightarrow{p})e ^{-i \overrightarrow{p} \cdot (\overrightarrow{x} - \overrightarrow{y})} \bigg] \\
    &= \sum_{\alpha = 1}^{4}\sum_{\beta = 1}^{4} \int \frac{d ^{3} p}{(2 \pi) ^{3}} \frac{1}{{2 E _{\overrightarrow{p}}}} \bigg[ u _{\alpha}(\overrightarrow{p})\overline{u}^{\dagger} _{\beta} \gamma ^{0} _{\alpha \beta}(\overrightarrow{p})e ^{i \overrightarrow{p} \cdot (\overrightarrow{x} - \overrightarrow{y})} +  v _{\alpha}(\overrightarrow{p})\overline{v}^{\dagger} _{\beta} \gamma ^{0} _{\alpha \beta}(\overrightarrow{p})e ^{-i \overrightarrow{p} \cdot (\overrightarrow{x} - \overrightarrow{y})} \bigg] \\
    &= \sum_{\alpha = 1}^{4}\sum_{\beta = 1}^{4} \int \frac{d ^{3} p}{(2 \pi) ^{3}} \frac{1}{{2 E _{\overrightarrow{p}}}} \bigg[ [(\gamma \cdot k + m)\gamma ^{0} ]_{\alpha \beta}(\overrightarrow{p})e ^{i \overrightarrow{p} \cdot (\overrightarrow{x} - \overrightarrow{y})} + [(\gamma \cdot k - m)\gamma ^{0} ]_{\alpha \beta} e ^{-i \overrightarrow{p} \cdot (\overrightarrow{x} - \overrightarrow{y})} \bigg] \\
\end{align*}

because
beacause of antiparticle

Therefore 
\begin{align*}
    &\left\{ \psi _{\alpha} (\overrightarrow{x}) , \psi ^{\dagger} _{\beta }(\overrightarrow{y})  \right\} =  \delta _{\alpha \beta} \delta ^{(3)} (\overrightarrow{x} - \overrightarrow{y})
\end{align*}
\end{document}
